further improve shal. emb. array reasoning support

isa/Gencot_CArray_Lemmas.thy
@@ -10,7 +10,7 @@ consts
   arr :: "'el list \<Rightarrow> 'arr"
   siz :: "'arr \<Rightarrow> nat"
   vld :: "'arr \<Rightarrow> nat \<Rightarrow> bool"
-  elm :: "'arr \<Rightarrow> nat \<Rightarrow> 'el"
+  elm :: "nat \<Rightarrow> 'arr \<Rightarrow> 'el"
   elm_update :: "nat \<Rightarrow> ('el \<Rightarrow> 'el) \<Rightarrow> 'arr \<Rightarrow> 'arr"
   elm_modified :: "nat \<Rightarrow> ('el \<Rightarrow> 'el \<Rightarrow> bool) \<Rightarrow> 'arr \<Rightarrow> 'arr \<Rightarrow> bool"
   arr_fill :: "(nat \<Rightarrow> 'el) \<Rightarrow> 'arr"
@@ -39,13 +39,13 @@ definition sizFxd :: "'arr \<Rightarrow> nat"
   where "sizFxd a \<equiv> length (lstFxd a)"
 definition vldFxd :: "'arr \<Rightarrow> nat \<Rightarrow> bool"
   where "vldFxd a i \<equiv> i < sizFxd a"
-definition elmFxd :: "'arr \<Rightarrow> nat \<Rightarrow> 'el"
-  where "elmFxd a i \<equiv> nth (lstFxd a) i"
+definition elmFxd :: "nat \<Rightarrow> 'arr \<Rightarrow> 'el"
+  where "elmFxd i a \<equiv> nth (lstFxd a) i"
 definition elm_updateFxd :: "nat \<Rightarrow> ('el \<Rightarrow> 'el) \<Rightarrow> 'arr \<Rightarrow> 'arr"
-  where "elm_updateFxd i f a \<equiv> arrFxd (list_update (lstFxd a) i (f (elmFxd a i)))"
+  where "elm_updateFxd i f a \<equiv> arrFxd (list_update (lstFxd a) i (f (elmFxd i a)))"
 definition elm_modifiedFxd :: "nat \<Rightarrow> ('el \<Rightarrow> 'el \<Rightarrow> bool) \<Rightarrow> 'arr \<Rightarrow> 'arr \<Rightarrow> bool"
   where elm_modified_def: "elm_modifiedFxd i m a1 a2 \<equiv> 
-    m (elmFxd a1 i) (elmFxd a2 i) \<and> (\<forall>j \<noteq> i. vldFxd a1 j \<longrightarrow> elmFxd a1 j = elmFxd a2 j)"
+    m (elmFxd i a1) (elmFxd i a2) \<and> (\<forall>j \<noteq> i. vldFxd a1 j \<longrightarrow> elmFxd j a1 = elmFxd j a2)"
 definition arr_fillFxd :: "(nat \<Rightarrow> 'el) \<Rightarrow> 'arr"
   where "arr_fillFxd f \<equiv> arrFxd [f x . x \<leftarrow> [0 ..< LENGTH('n)]]"
 
@@ -62,36 +62,49 @@ lemma sizArr: "sizFxd a = LENGTH('n)"
   by (simp add: length_FixedList)
 lemma vldArr: "vldFxd a n = (n < LENGTH('n))"
   by (simp add: vldFxd_def sizArr)
-lemma elmUpdElm: "elm_updateFxd i (f \<circ> (\<lambda>_. g (elmFxd a i))) a = elm_updateFxd i (f \<circ> g) a"
-  by (simp add: elm_updateFxd_def)
-lemma elmUpdDistrib: "(i < LENGTH('n)) \<Longrightarrow> elm_updateFxd i (f \<circ> g) = (elm_updateFxd i f) \<circ> (elm_updateFxd i g)"
+lemma elm_identUpd[simp]: "elm_updateFxd i (\<lambda>a. a) = (\<lambda>a. a)"
+  apply (unfold elm_updateFxd_def)
+  by(simp add: elmFxd_def arrFxd_def lstFxd_def Rep_FixedList_inverse fld_inverse)
+lemma elm_sameUpd: "elm_updateFxd i (\<lambda>_. m (elmFxd i x)) x = elm_updateFxd i m x"
+  by(simp add: elm_updateFxd_def)
+lemma elm_distUpd: "(i < LENGTH('n)) \<Longrightarrow> (elm_updateFxd i f) \<circ> (elm_updateFxd i g) = elm_updateFxd i (f \<circ> g)"
   for f:: "'el \<Rightarrow> 'el"
   apply (unfold elm_updateFxd_def elmFxd_def arrFxd_def lstFxd_def)
-  apply(rule ext)
-  apply(auto)
+  apply(rule ext,simp)
   apply(cut_tac x = "(fld a)" in Rep_FixedList )
   apply(subst wrp_inverse)+
   apply(subst Abs_FixedList_inverse,simp)+
   by(auto)
-lemma elmElmUpd: "vldFxd a i \<Longrightarrow> elmFxd (elm_updateFxd i f a) i = f (elmFxd a i)"
+lemma elm_commUpd_elm: "i < j \<Longrightarrow> (elm_updateFxd j m2) \<circ> (elm_updateFxd i m1) = (elm_updateFxd i m1) \<circ> (elm_updateFxd j m2)"
+  apply (unfold elm_updateFxd_def elmFxd_def arrFxd_def lstFxd_def)
+  apply(rule ext,simp)
+  apply(cut_tac x = "(fld x)" in Rep_FixedList )
+  apply(subst wrp_inverse)+
+  apply(subst Abs_FixedList_inverse,simp)+
+  apply (simp)
+  apply(rule arg_cong[where f=wrp])
+  apply(rule arg_cong[where f=Abs_FixedList])
+  apply(rule list_update_swap)
+  by(simp)
+lemma elmElmUpd: "vldFxd a i \<Longrightarrow> elmFxd i (elm_updateFxd i f a) = f (elmFxd i a)"
   apply(auto simp add: elm_updateFxd_def elmFxd_def arrFxd_def lstFxd_def vldArr)
   apply(cut_tac x = "(fld a)" in Rep_FixedList )
   apply(subst wrp_inverse)
   apply(subst Abs_FixedList_inverse)
   by (auto)
-lemma elmElmUpdFrame: "vldFxd a i \<and> vldFxd a j \<and> i \<noteq> j \<Longrightarrow> elmFxd (elm_updateFxd i f a) j = elmFxd a j"
+lemma elmElmUpdFrame: "vldFxd a i \<and> vldFxd a j \<and> i \<noteq> j \<Longrightarrow> elmFxd j (elm_updateFxd i f a) = elmFxd j a"
   apply(auto simp add: elm_updateFxd_def elmFxd_def arrFxd_def lstFxd_def vldArr)
   apply(cut_tac x = "(fld a)" in Rep_FixedList )
   apply(subst wrp_inverse)
   apply(subst Abs_FixedList_inverse)
   by (auto)
-lemma elmArrFill: "i < LENGTH('n) \<Longrightarrow> elmFxd (arr_fillFxd f) i = f i"
+lemma elmArrFill: "i < LENGTH('n) \<Longrightarrow> elmFxd i (arr_fillFxd f) = f i"
   apply(auto simp add: elmFxd_def arr_fillFxd_def lstFxd_def arrFxd_def wrp_inverse vldArr sizArr)
   apply(subst Abs_FixedList_inverse)
   by auto
 
 text \<open>Array equality by extensionality. \<close>
-lemma eqArr1: "(\<And> i. (vldFxd a1 i) \<Longrightarrow> ((elmFxd a1 i) = (elmFxd a2 i))) \<Longrightarrow> (a1 = a2)"
+lemma eqArr1: "(\<And> i. (vldFxd a1 i) \<Longrightarrow> ((elmFxd i a1) = (elmFxd i a2))) \<Longrightarrow> (a1 = a2)"
   apply(auto simp add: elmFxd_def vldFxd_def sizFxd_def lstFxd_def)
   apply(drule nth_equalityI[rotated])
   apply(cut_tac x = "(fld a1)" in Rep_FixedList )
@@ -103,7 +116,7 @@ lemma eqArr1: "(\<And> i. (vldFxd a1 i) \<Longrightarrow> ((elmFxd a1 i) = (elmF
   apply(simp add: fld_inverse)
   done
 lemma eqArr: "(a1 = a2) = 
-              (\<forall> i. (vldFxd a1 i) \<longrightarrow> ((elmFxd a1 i) = (elmFxd a2 i)))"
+              (\<forall> i. (vldFxd a1 i) \<longrightarrow> ((elmFxd i a1) = (elmFxd i a2)))"
   apply(rule iffI)
    apply(rule allI)
    apply(rule impI)
@@ -111,7 +124,7 @@ lemma eqArr: "(a1 = a2) =
   by (rule eqArr1,auto)
 
 lemma eqElmUpd: "vldFxd a2 i \<Longrightarrow> (a1 = elm_updateFxd i f a2) =
-                 ((elmFxd a1 i) = f (elmFxd a2 i) \<and> (\<forall> j. j \<noteq> i \<and> (vldFxd a1 j) \<longrightarrow> (elmFxd a1 j) = (elmFxd a2 j)))"
+                 ((elmFxd i a1) = f (elmFxd i a2) \<and> (\<forall> j. j \<noteq> i \<and> (vldFxd a1 j) \<longrightarrow> (elmFxd j a1) = (elmFxd j a2)))"
   apply(rule iffI)
    apply(auto)
     apply(subst elmElmUpd,auto)
@@ -126,7 +139,7 @@ lemma eqElmUpd: "vldFxd a2 i \<Longrightarrow> (a1 = elm_updateFxd i f a2) =
   done
 
 lemma eqArrFill: "(a = arr_fillFxd f) = 
-                 ((\<forall> i. (vldFxd a i) \<longrightarrow> ((elmFxd a i) = f i)))"
+                 ((\<forall> i. (vldFxd a i) \<longrightarrow> ((elmFxd i a) = f i)))"
   apply(rule iffI)
    apply(auto)
    apply(rule elmArrFill)
@@ -144,11 +157,11 @@ definition ctrct_getArrFxd :: "'arr \<times> ('m::len) word \<Rightarrow> bool"
   "ctrct_getArrFxd x \<equiv> let (a,i) = x in vldFxd a (unat i)"
 theorem sem_getArr: 
  "ctrct_getArrFxd (a,i) \<Longrightarrow> 
-  getArrFxd (a,i) = elmFxd a (unat i)"
+  getArrFxd (a,i) = elmFxd (unat i) a"
   by (simp add: getArrFxd_def getArr'_def vldArr elmFxd_def lstFxd_def)
 theorem errsem_getArr:
  "\<not> ctrct_getArrFxd (a,i) \<Longrightarrow> 
-  getArrFxd (a,i) = elmFxd a 0"
+  getArrFxd (a,i) = elmFxd 0 a"
   apply(simp add: getArrFxd_def getArr'_def vldArr elmFxd_def)
   apply(fold lstFxd_def)
   apply(case_tac " lstFxd a")
@@ -173,7 +186,7 @@ definition ctrct_modifyArrFxd :: "'arr \<times> ('m::len) word \<times> ('el \<t
 theorem sem_modifyArr:
  "ctrct_modifyArrFxd (a,i,f,x) \<Longrightarrow> 
   modifyArrFxd (a,i,f,x) = 
-  (let (e,y) = f (elmFxd a (unat i), x) in (elm_updateFxd (unat i) (\<lambda>_.e) a, y))"
+  (let (e,y) = f (elmFxd (unat i) a, x) in (elm_updateFxd (unat i) (\<lambda>_.e) a, y))"
   by (simp add: modifyArrFxd_def modifyArr'_def split_def Let_def vldArr lstFxd_def arrFxd_def elm_updateFxd_def elmFxd_def)
 theorem errsem_modifyArr:
  "\<not> ctrct_modifyArrFxd (a,i,f,x) ==> 
@@ -186,12 +199,38 @@ definition ctrct_modifyArrDfltFxd :: "'arr \<times> ('m::len) word \<times> ('el
 theorem sem_modifyArrDflt:
  "ctrct_modifyArrDfltFxd (a,i,f,x) ==> 
   modifyArrDfltFxd (a,i,f,x) = 
-  (let (e,y) = f (elmFxd a (unat i), x) in (elm_updateFxd (unat i) (\<lambda>_.e) a, y))"
+  (let (e,y) = f (elmFxd (unat i) a, x) in (elm_updateFxd (unat i) (\<lambda>_.e) a, y))"
   by (simp add: modifyArrDfltFxd_def modifyArrDflt'_def split_def Let_def vldArr lstFxd_def arrFxd_def elm_updateFxd_def elmFxd_def)
 theorem errsem_modifyArrDflt:
  "\<not> ctrct_modifyArrDfltFxd (a,i,f,x) ==>
   modifyArrDfltFxd (a,i,f,x) = (a, defaultVal ())"
   by (simp add: modifyArrDfltFxd_def modifyArrDflt'_def vldArr fld_inverse)
+
+definition ctrct_modrefArrFxd :: "'arr \<times> ('m::len) word \<times> ('pel \<times> 'arg \<Rightarrow> 'pel \<times> 'arg) \<times> 'arg \<Rightarrow> bool"
+  where ctrct_modrefArrFxd_def[simp]:
+  "ctrct_modrefArrFxd x \<equiv> let (a,i,f,v) = x in vldFxd a (unat i)"
+theorem sem_modrefArr:
+ "ctrct_modrefArrFxd (a,i,f,x) \<Longrightarrow> 
+  modrefArrFxd (a,i,f,x) = 
+  (let (e,y) = f (toPtr (elmFxd (unat i) a), x) in (elm_updateFxd (unat i) (\<lambda>_.frPtr e) a, y))"
+  by (simp add: modrefArrFxd_def modrefArr'_def split_def Let_def vldArr lstFxd_def arrFxd_def elm_updateFxd_def elmFxd_def)
+theorem errsem_modrefArr:
+ "\<not> ctrct_modrefArrFxd (a,i,f,x) ==> 
+  modrefArrFxd (a,i,f,x) = (a, x)"
+  by (simp add: modrefArrFxd_def modrefArr'_def vldArr fld_inverse)
+
+definition ctrct_modrefArrDfltFxd :: "'arr \<times> ('m::len) word \<times> ('pel \<times> 'arg \<Rightarrow> 'pel \<times> 'out) \<times> 'arg \<Rightarrow> bool"
+  where ctrct_modrefArrDfltFxd_def[simp]:
+  "ctrct_modrefArrDfltFxd x \<equiv> let (a,i,f,v) = x in vldFxd a (unat i)"
+theorem sem_modrefArrDflt:
+ "ctrct_modrefArrDfltFxd (a,i,f,x) ==> 
+  modrefArrDfltFxd (a,i,f,x) = 
+  (let (e,y) = f (toPtr (elmFxd (unat i) a), x) in (elm_updateFxd (unat i) (\<lambda>_.frPtr e) a, y))"
+  by (simp add: modrefArrDfltFxd_def modrefArrDflt'_def split_def Let_def vldArr lstFxd_def arrFxd_def elm_updateFxd_def elmFxd_def)
+theorem errsem_modrefArrDflt:
+ "\<not> ctrct_modrefArrDfltFxd (a,i,f,x) ==>
+  modrefArrDfltFxd (a,i,f,x) = (a, defaultVal ())"
+  by (simp add: modrefArrDfltFxd_def modrefArrDflt'_def vldArr fld_inverse)
 
 end
 
